AwsCryptographicMaterialProviders/src/Keyrings/AwsKms/AwsKmsRsaKeyring.dfy
@@ -1,0 +1,86 @@
+// Copyright Amazon.com Inc. or its affiliates. All Rights Reserved.
+// SPDX-License-Identifier: Apache-2.0
+
+include "../../Keyring.dfy"
+include "../../Materials.dfy"
+
+include "../../../Model/AwsCryptographyMaterialProvidersTypes.dfy"
+
+module AwsKmsRsaKeyring {
+  import opened StandardLibrary
+  import opened Wrappers
+  import opened UInt = StandardLibrary.UInt
+  import Keyring
+  import Materials
+  import Types = AwsCryptographyMaterialProvidersTypes
+  import KMS = ComAmazonawsKmsTypes
+
+  class AwsKmsRsaKeyring
+    extends Keyring.VerifiableInterface
+  {
+
+    predicate ValidState()
+    ensures ValidState() ==> History in Modifies
+    {
+      && History in Modifies
+    }
+
+    constructor (
+      publicKey: Option<seq<uint8>>,
+      kmsKeyId: string,
+      encryptionAlgorithm: KMS.EncryptionAlgorithmSpec,
+      client: Option<KMS.IKeyManagementServiceClient>,
+      grantTokens: KMS.GrantTokenList
+    )
+      ensures ValidState() && fresh(this) && fresh(History)
+        && fresh(Modifies - (if client.Some? then client.value.Modifies else {}))
+    {
+      // TODO set up keyring
+
+      History := new Types.IKeyringCallHistory();
+      Modifies := {History};
+      if client.Some? {
+        Modifies := Modifies + client.value.Modifies;
+      }
+    }
+
+    predicate OnEncryptEnsuresPublicly ( input: Types.OnEncryptInput , output: Result<Types.OnEncryptOutput, Types.Error> ) {true}
+    
+    method OnEncrypt'(input: Types.OnEncryptInput)
+      returns (res: Result<Types.OnEncryptOutput, Types.Error>)
+      requires ValidState()
+      modifies Modifies - {History}
+      decreases Modifies - {History}
+      ensures ValidState()
+      ensures OnEncryptEnsuresPublicly(input, res)
+      ensures unchanged(History) 
+      ensures res.Success?
+      ==>
+        && Materials.ValidEncryptionMaterialsTransition(
+          input.materials,
+          res.value.materials
+        )
+    {
+      return Failure(Types.AwsCryptographicMaterialProvidersException(message := "Unimplemented"));
+    }
+
+     predicate OnDecryptEnsuresPublicly ( input: Types.OnDecryptInput , output: Result<Types.OnDecryptOutput, Types.Error> ) {true}
+    method OnDecrypt'(input: Types.OnDecryptInput)
+      returns (res: Result<Types.OnDecryptOutput, Types.Error>)
+      requires ValidState()
+      modifies Modifies - {History}
+      decreases Modifies - {History}
+      ensures ValidState()
+      ensures OnDecryptEnsuresPublicly(input, res)
+      ensures unchanged(History)
+      
+      ensures res.Success?
+      ==>
+        && Materials.DecryptionMaterialsTransitionIsValid(
+          input.materials,
+          res.value.materials)
+    {
+      return Failure(Types.AwsCryptographicMaterialProvidersException(message := "Unimplemented"));
+    }
+  }
+}
